\begin{answer}
\newline
First calculate first partial derivative:
\begin{equation*}
	\begin{aligned}
		\frac{ \partial J ( \theta )}{\partial \theta _j} &= -\frac{1}{m} \sum_{i=1}^m y^{(i)} \frac{1}{h_\theta(x^{(i)})}\frac{\partial}{\partial \theta _j}h_\theta (x^{(i)}) + (1-y^{(i)}) \frac{1}{1-h_\theta(x^{(i)})}\frac{\partial}{\partial \theta _j}(1-h_\theta(x^{(i)}) ) \\
		&= -\frac{1}{m} \sum_{i=1}^m y^{(i)} \frac{1}{g(\theta ^T x^{(i)})}\frac{\partial}{\partial \theta _j}h_\theta (x^{(i)}) + (1-y^{(i)}) \frac{1}{1-g(\theta ^T x^{(i)})}\frac{\partial}{\partial \theta _j}(1-g(\theta ^T x^{(i)}) ) \\
		&= -\frac{1}{m} \sum_{i=1}^{m}  y^{(i)} \left[1 - g(\theta^T x^{(i)})\right]x^{(i)}_j - (1 - y^{(i)}) g(\theta^T x^{(i)})x^{(i)}_j  \\
		&= \frac{1}{m} \sum_{i=1}^{m} \left[ g(\theta^T x^{(i)}) - y^{(i)} \right]x^{(i)}_j \\
	\end{aligned}
\end{equation*}
Therefore, we have the gradient:
\begin{equation*}
		\nabla _\theta J(\theta) = \frac{1}{m} X^T (g(X \theta) - Y )
\end{equation*}

Then calculate second partial derivative:

\begin{equation*}
		H_{jk} = \frac{\partial^2 J(\theta)}{\partial \theta_j \partial \theta_k} = \frac{1}{m} \sum_{i=1}^m g(\theta ^ T x^{(i)}) (1- g(\theta ^ T x^{(i)}) x_j ^{(i)} x_k ^ {(i)}
\end{equation*}
Hence getting the Hessian:
\begin{equation*}
	H = \frac{1}{m} [X^T g(X\theta) (1-g(X\theta))] X
\end{equation*}
To show that $z^THz \geq 0$, we can rewrite in this form:
\begin{equation*}
	\begin{aligned}
	z^T Hz &= \frac{1}{m} \sum_{i=1}^{m} \sum_{j=1}^{n} \sum_{k=1}^{n} g(\theta^T x^{(i)})[1 - g(\theta^T x^{(i)})]x_j^{(i)}x_k^{(i)}z_j z_k \\
	&= \frac{1}{m} \sum_{i=1}^{m} g(\theta^T x^{(i)})[1 - g(\theta^T x^{(i)})][(x^{(i)})^T z]^2 \geq 0	
	\end{aligned}
\end{equation*}

\end{answer}
